TamaProof.lean
@@ -1,4 +1,5 @@
 import TamaSpec
+import proof.OwnableProof
 import proof.ERC20Proof
 import proof.ERC721Proof
 import proof.WETHProof
