TamaSpec.lean
@@ -1,4 +1,5 @@
 import TamaSrc
+import spec.OwnableSpec
 import spec.ERC20Spec
 import spec.ERC721Spec
 import spec.WETHSpec
