TamaSrc.lean
@@ -1,3 +1,4 @@
+import src.Ownable
 import src.ERC20
 import src.ERC721
 import src.WETH
